lntrs.v
@@ -43,6 +43,7 @@ all : cycle 1.
 { nsgen_sw nsr rs sppc (l, l0, d) (Γ, Δ', d0) acm inps0 swap. }
 
 (* now case where move and rule application occur in the same sequent *)
+{
 injection H0 as. subst.
 inversion sppc as [? ? ? ? ? ? pr mse se].
 destruct c.
@@ -62,6 +63,7 @@ repeat ((list_eq_nc || (pose pr as Qpr ; apply roe in Qpr)) ;
   try (rewrite app_nil_r) ; try (rewrite app_nil_r in pr)) ;
 (* above produces 20 subgoals, following solves all of them!! *)
 nsprsameR princrules rs pr q qin inmps acm inps0 x0. 
+}
 
 Qed.
 
@@ -93,4 +95,82 @@ intros.  assumption.
 Qed.
 
 Check gen_swapR.
+
+(** now the same thing for left context only **)
+Lemma gen_swapR_step_roe_lc: forall V ps concl princrules
+  (last_rule rules : rls (list (rel (list (PropF V)) * dir))),
+  rules_R_oe princrules -> 
+  last_rule = nslcrule (seqrule princrules) ->
+  gen_swapR_step last_rule rules ps concl.
+Proof.  intros until 0.  unfold gen_swapR_step.
+intros roe lreq nsr drs acm rs. subst. clear drs.
+
+inversion nsr as [? ? ? ? sppc mnsp nsc].
+unfold nsext in nsc.
+rewrite can_gen_swapR_def'.  intros until 0. intros swap pp ss.
+unfold nslcext in pp.
+
+apply partition_2_2 in pp.
+
+destruct c.
+sE ; subst.
+
+{ nsgen_sw nsr rs sppc (l, l0, d) (Γ, Δ', d0) acm inps0 swap. }
+
+(* now case where move and rule application occur in the same sequent *)
+{
+injection H0 as. subst.
+inversion sppc as [? ? ? ? ? ? pr mse se].
+destruct c.
+unfold seqext in se.
+subst.  clear nsr. clear sppc.
+injection se as sel ser.
+subst.
+
+unfold rules_R_oe in roe.
+inversion_clear swap ; subst.
+
+(* do as much as possible for all rules at once *)
+acacD' ; (* gives 10 subgoals *)
+subst ;
+repeat ((list_eq_nc || (pose pr as Qpr ; apply roe in Qpr)) ;
+  sD ; subst ; simpl ; simpl in pr ;
+  try (rewrite app_nil_r) ; try (rewrite app_nil_r in pr)) ;
+(* above produces 20 subgoals, following solves all of them!! *)
+nsprsameR princrules rs pr q qin inmps acm inps0 x0. 
+}
+
+{ apply eq_sym in H1. list_eq_nc. contradiction. }
+
+Qed.
+
+Check gen_swapR_step_roe_lc.
+
+Lemma gen_swapR_step_pr_lc: forall V ps concl 
+  (last_rule rules : rls (list (rel (list (PropF V)) * dir))),
+  last_rule = nslcrule (seqrule (@princrule V)) ->
+  gen_swapR_step last_rule rules ps concl.
+Proof.  intros. eapply gen_swapR_step_roe_lc.
+  apply princrule_R_oe'. exact H. Qed.
+
+Check gen_swapR_step_pr_lc.
+
+Lemma gen_swapR_lc: forall {V : Set} ns
+  (D : derrec (nslcrule (seqrule (@princrule V))) (fun _ => False) ns),
+  can_gen_swapR (nslcrule (seqrule (@princrule V))) ns.
+
+Proof. 
+intro.  intro.  intro.
+eapply derrec_all_ind in D.
+exact D. tauto.
+intros. inversion H. 
+subst.
+pose gen_swapR_step_pr_lc.
+unfold gen_swapR_step in g.
+eapply g. reflexivity. eassumption. assumption. assumption.
+unfold rsub. clear g. 
+intros.  assumption.
+Qed.
+
+Check gen_swapR_lc.
 
